Further progress on new async read proof
More cleanup of definitions. Distinction between memory and ghost cache
makes many facts less obvious, and expressing them as lemmas suitable
for eauto (rather than for forward chaining) proves a challenge.

src/ConcurrentCache.v
@@ -740,6 +740,105 @@ Qed.
 
 Hint Resolve lock_protocol_same_cache.
 
+Definition mem_lock cl :=
+  match cl with
+  | Owned tid => Locked
+  | NoOwner => Open
+  end.
+
+Lemma cache_state_none : forall st (c: AssocCache st) (a:addr),
+    cache_state c a = None ->
+    cache_get c a = None.
+Proof.
+  intros.
+  rewrite cache_state_as_get in H.
+  case_cache_val.
+Qed.
+
+Lemma cache_val_as_get : forall st (c: AssocCache st) (a:addr),
+    cache_val c a =
+    match cache_get c a with
+    | Some (Clean v _) => Some v
+    | Some (Dirty v _) => Some v
+    | _ => None
+    end.
+Proof.
+  reflexivity.
+Qed.
+
+Lemma ghost_lock_invariant_functional : forall l gl,
+    ghost_lock_invariant l gl ->
+    l = mem_lock gl.
+Proof.
+  unfold mem_lock.
+  inversion 1; subst; congruence.
+Qed.
+
+Theorem cache_eq_mem : forall c c' (a:addr) oce,
+    cache_eq ghost_lock_invariant c c' ->
+    cache_get c' a = oce ->
+    cache_get c a =
+    match oce with
+    | Some (Clean v s) =>
+      Some (Clean v (mem_lock s))
+    | Some (Dirty v s) =>
+      Some (Dirty v (mem_lock s))
+    | Some (Invalid s) =>
+      Some (Invalid (mem_lock s))
+    | None => None
+    end.
+Proof.
+  unfold cache_eq.
+  intros; subst.
+  specific_addr; intuition.
+  inversion H;
+    try match goal with
+        | [ H: ghost_lock_invariant _ _ |- _ ] =>
+          pose proof (ghost_lock_invariant_functional H)
+        end; try inv_opt;
+    try congruence.
+Qed.
+
+Lemma cache_eq_open : forall c c' (a:addr),
+    cache_eq ghost_lock_invariant c c' ->
+    cache_state c' a = Some NoOwner ->
+    cache_state c a = Some Open.
+Proof.
+  intros.
+  eapply cache_eq_mem with (a := a) in H; eauto.
+  rewrite cache_state_as_get in *.
+  case_cache_val' c' a;
+    inv_opt; cbn;
+    congruence.
+Qed.
+
+Lemma cache_eq_invalid : forall c c' (a:addr) tid,
+    cache_eq ghost_lock_invariant c c' ->
+    gcache_get_lock c' a = Owned tid ->
+    cache_get c a = Some (Invalid Locked) ->
+    cache_get c' a = Some (Invalid (Owned tid)).
+Proof.
+  unfold gcache_get_lock.
+  intros.
+  rewrite cache_state_as_get in *.
+  case_cache_val;
+    eapply cache_eq_mem with (a := a) in H;
+    eauto;
+    subst; congruence.
+Qed.
+
+Hint Resolve diskIs_same.
+
+Lemma addr_val_is : forall AT AEQ V (m: @mem AT AEQ V) a v,
+    m a = Some v ->
+    (diskIs (mem_except m a) * a |-> v)%pred m.
+Proof.
+  intros.
+  eapply diskIs_combine_same'; eauto.
+Qed.
+
+Hint Resolve addr_val_is.
+
 Theorem locked_AsyncRead_ok : forall a,
   stateS TID: tid |-
   {{ F v rest,
@@ -793,22 +892,18 @@ Proof.
   unfold get_scache_val, opt_cache_entry_val in H16.
   simpl_get_set in H16.
   assert (cache_get (get GCache s) a = Some (Invalid (Owned tid))).
-  (* need lemmas for using cache_eq to derive equalities from ghost
-  contents to mem contents *)
-  admit.
+  eauto using cache_eq_invalid.
+
+  assert (cache_get (get Cache m0) a = Some (Invalid Locked)).
+  eapply cache_eq_mem in H21; eauto; simplify.
+  eauto.
+  assert (get GDisk s2 a = d1 a) by eauto using cache_miss_mem_eq.
+  assert (d1 a = Some (Valuset v rest, Some tid)) by eauto.
+  eapply addr_val_is; eauto.
 
   time "step" step pre (time "simplify" simplify) with finish.
 
-  step pre simplify with idtac.
-  (* BUG: finish gives "Conversion test raised an anomaly" *)
-  rewrite H28.
-  autorewrite with upd.
-  solve_global_transitions; eauto;
-  try solve_modified;
-  try congruence.
-  assert (d1 = upd d a (Valuset v rest, None)).
-  eapply diskIs_combine_upd in H1; eauto.
-  subst.
+  step pre simplify with finish.
 
   all: repeat match goal with
          | [ H: cache_get ?c ?a = None, H': ?c' = ?c |- _ ] =>
@@ -820,28 +915,6 @@ Proof.
        | [ H: cache_get ?c _ = None, H': cache_pred ?c _ _ |- _ ] =>
          learn that (cache_miss_mem_eq _ H' H)
        end.
-  assert (d a = Some (Valuset v rest, None)) by auto.
-  autorewrite with upd.
-  eauto.
-
-  rewrite H28.
-  autorewrite with upd; now auto.
-  rewrite H28.
-  autorewrite with upd.
-  (* relation between s and s'; theorem statement is currently
-  broken *)
-  admit.
-
-  rewrite H28.
-  autorewrite with upd.
-  eapply star_one_step.
-  finish.
-  case_eq (weq a0 a); intros; subst; eauto.
-  eexists; eauto.
-  eapply equal_f in H28.
-  rewrite H47 in H28.
-  autorewrite with upd in H28.
-  eauto.
 Admitted.
 
 Hint Extern 4 {{ locked_AsyncRead _; _ }} => apply locked_AsyncRead_ok : prog.
